user 5, session 19, part 9

diffs-w-failures-no-compiles/5/user-5-session-19.v
@@ -1,5 +1,7 @@
 Require Import String.
 Require Import ZArith.
+Require Import List.
+Import ListNotations.
 Definition Identifier := string.
 Definition id_eq_dec := string_dec.
 Inductive Term : Set :=
@@ -115,3 +117,29 @@ symmetry.
 (apply evalEqFalse).
 assumption.
 Admitted.
+Fixpoint free_vars (t : Term) : list Identifier :=
+  match t with
+  | Var x => [x]
+  | Int _ => []
+  | Eq a b => free_vars a ++ free_vars b
+  | Plus a b => free_vars a ++ free_vars b
+  | Times a b => free_vars a ++ free_vars b
+  | Minus a b => free_vars a ++ free_vars b
+  | Choose x P =>
+      filter (fun y => if id_eq_dec x y then false else true) (free_vars P)
+  end.
+Axiom (fresh_var : list Identifier -> Identifier).
+Axiom (fresh_var_unique : forall exclude, ~ In (fresh_var exclude) exclude).
+Definition Divide (t1 : Term) (t2 : Term) :=
+  let x := fresh_var (free_vars t1 ++ free_vars t2) in
+  Choose x (Eq t1 (Times (Var x) t2)).
+Lemma divide_test :
+  forall L env, L.(eval) env (Divide (Int 6) (Int 2)) = L.(eval) env (Int 3).
+Proof.
+(intros).
+(unfold Divide).
+(match goal with
+ | |- context [ Choose ?x _ ] => generalize x
+ end).
+intro x.
+(rewrite evalChoose).
